+++
date = "2017-11-06T12:16:53+08:00"
title = "2.6 Chain Rule"
+++

# 2.6 Chain Rule

The Chain Rule is more general than the Inverse Function Rule and deals with the case where \\(x\\) and \\(y\\) are both functions of a third variable \\(t\\).

Suppose

$$
x = f(t), y = G(x).
$$

Thus \\(x\\) depends on \\(t\\), and \\(y\\) depends on \\(x\\). But \\(y\\) is also a function of \\(t\\),

$$
y = g(t),
$$

where \\(g\\) is defined by the rule

$$
g(t) = G(f(t)).
$$

The function \\(g\\) is sometimes called the _composition_ of \\(G\\) and \\(f\\) (sometimes written \\(g = G \circ f\\)).

The composition of \\(G\\) and \\(f\\) may be described in terms of black boxes. The function \\(g = G \circ f\\) is a large black box operating on the input \\(t\\) to produce \\(g(t) = G(f(t))\\). If we look inside this black box (pictured in Figure 2.6.1), we see two smaller black boxes, \\(f\\) and \\(G\\). First \\(f\\) operates on the input \\(t\\) to produce \\(f(t)\\), and then \\(G\\) operates on \\(f(t)\\) to produce the final output \\(g(t) = G(f(t))\\).

The Chain Rule expresses the derivative of \\(g\\) in terms of the derivatives of \\(f\\) and \\(G\\). It leads to the powerful method of "change of variables" in computing derivatives and, later on, integrals.

![figure 2.6.1](/calculus/img/keisler/f2.6.1.gif)

**Figure 2.6.1**

## CHAIN RULE

_Let \\(f\\), \\(G\\) be two real functions and define the new function \\(g\\) by the rule_

$$
g(t) = G(f(t)).
$$

_At any value of \\(t\\) where the derivatives \\(f^\prime(t)\\) and \\(G^\prime(f(t))\\) exist, \\(g^\prime(t)\\) also exists and has the value_

$$
g^\prime(t) = G^\prime(f(t))f^\prime(t).
$$

### PROOF

Let

$$
x = f(t),\ \ y = g\(t),\ \ y = G(x).
$$

Take \\(t\\) as the independent variable, and let \\(\Delta{f} \ne 0\\) be infinitesimal. Form the corresponding increments \\(\Delta{x}\\) and \\(\Delta{y}\\). By the Increment Theorem for \\(x = f(t)\\), \\(\Delta{x}\\) is infinitesimal. Using the Increment Theorem again but this time for \\(y = G(x)\\), we have

$$
\Delta{y} = G^\prime(x)\ \Delta{x} + \varepsilon\ \Delta{x}
$$

for some infinitesimal \\(\varepsilon\\). Dividing by \\(\Delta{t}\\),

$$
\frac{\Delta{y}}{\Delta{t}} = G^\prime(x)\frac{\Delta{x}}{\Delta{t}} + \varepsilon\frac{\Delta{x}}{\Delta{t}}.
$$

Then taking standard parts,

$$
st\Bigl(\frac{\Delta{y}}{\Delta{t}}\Bigr) = G^\prime(x)st\Bigl(\frac{\Delta{x}}{\Delta{t}}\Bigr) + 0,
$$

or

$$
g^\prime(t) = G^\prime(x)f^\prime(t) = G^\prime(f(t))f^\prime(t).
$$

### EXAMPLE 1

Find the derivative of \\(g(t) = \ln\ (\sin t)\\). \\(g(t)\\) is the natural logarithm of the sine of \\(t\\). It can be written in the form

$$
g(t) = G(f(t))
$$

where

$$
f(t) = \sin t,\ \ G(x) = \ln x.
$$

We have

$$
f^\prime(t) = \cos t,\ \ G^\prime(x) = \frac{1}{x}.
$$

By the Chain Rule,

$$
g^\prime(t) = G^\prime(f(t))f^\prime(t)
$$

$$
= \frac{1}{\sin t} \cdot \cos t = \frac{\cos t}{\sin t}.
$$

### EXAMPLE 2

Find the derivative of \\(g(t) = \sqrt{3t + 1}\\). \\(g(t)\\) has the form

$$
g(t) = G(f(t)),
$$

where

$$
f(t) = 3t + 1,\ \ G(x) = \sqrt(x).
$$

We have

$$
f^\prime(t) = 3, G^\prime(x) = \frac{1}{2}x^{-1 / 2}.
$$

Then

$$
g^\prime(t) = G^\prime(f(t))f^\prime(t)
$$

$$
= \frac{1}{2}(3t + 1)^{-1 / 2}3 = \frac{3}{2\sqrt{3t + 1}}.
$$

In practice it is more convenient to use the Chain Rule with dependent variables \\(x\\) and \\(y\\) instead of functions \\(f\\) and \\(g\\).

## CHAIN RULE WITH DEPENDENT VARIABLES

_Let_

$$
x = f(t),\ \ y = g(t) = G(x).
$$

_Assume \\(g^\prime(t)\\) and \\(G^\prime(x)\\) exist. Then_

$$
(i)\ \ \frac{dy}{dt} = \frac{dy}{dx}\frac{dx}{dt}
$$

$$
(ii)\ \ dy = \frac{dy}{dx}dx
$$

_where \\(dx/dt\\), \\(dy/dt\\) are computed with \\(t\\) as the independent variable, and \\(dy/dx\\) is computed with \\(x\\) as the independent variable._

Let us work Examples 1 and 2 again with dependent variables.

### EXAMPLE 1 (Continued)

Let \\(x = \sin t\\), \\(y = \ln x\\).

Find \\(dy/dt\\) using Chain Rule (i) and \\(d\\)y by using Chain Rule (ii).

(i)

$$
\frac{dx}{dt} = \cos t,\ \ \frac{dy}{dx} = \frac{1}{x},
$$

$$
\frac{dy}{dt} = \frac{dy}{dx} \cdot \frac{dx}{dt} = \frac{1}{x} \cdot \cos t = \frac{\cos t}{\sin t}.
$$

(ii)

$$
dx = \cos t\ dt,\ \ \frac{dy}{dx} = \frac{1}{x},
$$

$$
dy = \frac{1}{x}dx = \frac{1}{x}\cos t\ dt = \frac{\cos t}{\sin t}\ dt.
$$

### EXAMPLE 2 (Continued)

Let \\(x = 3t + 1\\), \\(y = \sqrt{x}\\).

(i)

$$
\frac{dx}{dt} = 3, \ \ \frac{dy}{dx} = \frac{1}{2}x^{-1 / 2},
$$

$$
\frac{dy}{dt} = \frac{dy}{dx}\frac{dx}{dt} = \frac{3}{2}x^{-1 / 2} = \frac{3}{2}(3t + 1)^{-1 / 2}.
$$

(ii)

$$
dx = 3\ dt, \ \ \frac{dy}{dx} = \frac{1}{2}x^{-1 / 2},
$$

$$
dy = \frac{1}{2}x^{-1 / 2}\ dx = \frac{1}{2}(3t + 1)^{-1 / 2}3\ dt
$$

$$
= \frac{3}{2}(3t + 1)^{-1 / 2}\ dt.
$$

The equation

$$
\frac{dy}{dt} = \frac{dy}{dx}\frac{dx}{dt}
$$

with \\(t\\) as the independent variable is trivial. We simply cancel the \\(dx\\)'s. But when \\(dy/dx\\) is computed with \\(x\\) as the independent variable while \\(dx/dt\\) is computed with \\(t\\) as the independent variable, the two \\(dx\\)'s have different meanings, and the equation is not trivial.

Similarly, the equation

$$
dy = \frac{dy}{dx}dx
$$

is trivial with \\(x\\) as the independent variable but not when \\(t\\) is the independent variable in \\(dy\\) and \\(dx\\), while \\(x\\) is independent in \\(dy/dx\\).

The Chain Rule shows that when we change independent variables the equations

$$
\frac{dy}{dt} = \frac{dy}{dx}\frac{dx}{dt}, \ \ dy = \frac{dy}{dx}dx
$$

remain true.

The Inverse Function Rule can be proved from the Chain Rule as follows.

Let

$$
y = f(x), \ \ x = g(y)
$$

be inverse functions whose derivatives exist. Then

$$
\frac{dy}{dx}\frac{dx}{dy} = \frac{dy}{dy} = 1,
$$

whence

$$
\frac{dy}{dx} = \frac{1}{dx/dy}, \ \ f^\prime(x) = \frac{1}{g^\prime(y)}.
$$

Using the Chain Rule we may write the Power Rule in a general form.

## POWER RULE

_Let \\(r\\) be a rational number, and let \\(u\\) depend on \\(x\\). If \\(u > 0\\) and \\(du/dx\\) exists, then_

$$
\frac{d(u^r)}{dx} = ru^{r-1}\frac{du}{dx}.
$$

This is proved by letting \\(y = u^r\\) and computing \\(dy/dx\\) by the Chain Rule,

$$
\frac{dy}{dx} = \frac{dy}{du}\frac{du}{dx} = ru^{r-1}\frac{du}{dx}.
$$

The Chain Rule has two types of applications.

(1) Given \\(x = f(t)\\) and \\(y = G(x)\\), find \\(\frac{dy}{dt}\\). Use \\(\frac{dy}{dt} = \frac{dy}{dx}\frac{dx}{dt}\\).

(2) Given \\(x = f(t)\\) and \\(y = g(t)\\), find \\(\frac{dy}{dx}\\). Use \\(\frac{dy}{dx} = \frac{dy/dt}{dx/dt}\\).

Applications of type (1) often arise when a new dependent variable \\(x\\) is introduced to help compute \\(\frac{dy}{dt}\\). Applications of type (2) arise when two variables \\(x\\) and \\(y\\) both depend on a third variable \\(t\\), for example, when \\(x\\) and \\(y\\) are the coordinates of a moving particle and \\(t\\) is time.

We give three examples of type (1) and then two of type (2).

### EXAMPLE 3

Suppose that by investing \\(t\\) dollars a company can produce

$$
x = \frac{t}{10} - 100, \ \ t \ge 1000,
$$

items, and that it can sell \\(x\\) items for a total profit of

$$
y = 5x - \frac{x^2}{100}.
$$

Find \\(\frac{dy}{dt}\\), which is the marginal profit with respect to the amount invested.

We have

$$
\frac{dx}{dt} = \frac{1}{10},\ \ \frac{dy}{dx} = 5 - \frac{x}{50}.
$$

By the Chain Rule,

$$
\frac{dy}{dt} = \frac{dy}{dx}\frac{dx}{dt} = \Bigl(5 - \frac{x}{50}\Bigr)\frac{1}{10}
$$

$$
= \Bigl(5 - \frac{\frac{t}{10} - 100}{50}\Bigr)\frac{1}{10}
$$

$$
= 0.7 - \frac{t}{5000}.
$$

Thus after \\(t\\) dollars have been invested, an additional dollar invested will bring 0.7 â€” \\(t\\)/5000 dollars of additional profit.

### EXAMPLE 4

Find \\(dy/dt\\) where \\(y = (5t^2 - 2)^{1 / 4}\\).

Let

$$
x = 5t^2 - 2,\ \ y = x^{1 / 4}.
$$

Then

$$
\frac{dx}{dt} = 10t, \ \ \frac{dy}{dx} = \frac{1}{4}x^{-3 / 4},
$$

$$
\frac{dy}{dt} = \frac{dy}{dt}\frac{dx}{dt} = \Bigl(\frac{1}{4}x^{-3 / 4}\Bigr)(10t)
$$

$$
= \frac{10}{4}(5t^2 - 2)^{-3 / 4}t.
$$

### EXAMPLE 5

Find \\(dy/dx\\) where \\(y = \sqrt{\sin(4x + 1) + \cos(4x - 1)}\\). This problem requires three uses of the Chain Rule.

Let 

$$
u = \sin (4x + 1) + \cos (4x - 1),
$$

$$
y = \sqrt{u}.
$$

Then by the Chain Rule,

$$
\frac{dy}{dx} = \frac{dy}{du} \cdot \frac{du}{dx} = \frac{1}{2\sqrt{u}} \cdot \frac{du}{dx}.
$$

Now let

$$
v = \sin(4x + 1),
$$

$$
w = \cos(4x - 1),
$$

$$
u = v + w.
$$

Then

$$
\frac{du}{dx} = \frac{dv}{dx} + \frac{dw}{dx}.
$$

We use the Chain Rule twice more to find \\(dv/dx\\) and \\(dw/dx\\).

$$
v = \sin (4x + 1).
$$

$$
\frac{dv}{dx} = \cos (4x + 1)\frac{d(4x + 1)}{dx}
$$

$$
 = 4\cos (4x + 1).
$$

$$
w = \cos (4x - 1).
$$

$$
\frac{dw}{dx} = -\sin (4x - 1)\frac{d(4x - 1)}{dx}
$$

$$
= -4\sin (4x - 1).
$$

Finally, we combine everything to get

$$
\frac{dy}{dx} = \frac{1}{2\sqrt{u}} \cdot \frac{du}{dx} = \frac{1}{2\sqrt{u}}\Bigl(\frac{dv}{dx} + \frac{dw}{dx}\Bigr)
$$

$$
= \frac{4\cos (4x + 1) - 4\sin(4x - 1)}{2\sqrt{\sin(4x + 1) + \cos(4x - 1)}}.
$$

If a particle is moving in the plane, its position \\((x, y)\\) at time \\(t\\) will be given by a pair of equations

$$
x = f(t),\ \ y = g(t).
$$

These are called _parametric equations_. The slope of the curve traced out by this particle can be found by the Chain Rule,

$$
\frac{dy}{dx} = \frac{dy/dt}{dx/dt} = \frac{g^\prime(t)}{f^\prime{t}},
$$

whenever the derivatives exist and \\(f^\prime(t) \ne 0\\). This is a Chain Rule application of type (2).

### EXAMPLE 6

A ball thrown horizontally from a 100 ft cliff at a velocity of 50 ft/sec will follow the parametric equations

$$
x = 50t,\ \ y = 100 - 16t^2,
$$

in feet. Find the slope of its path at time \\(t\\) (Figure 2.6.2).

$$
\frac{dx}{dt} = 50,\ \ \frac{dy}{dt} = -32t,
$$

so

$$
\frac{dy}{dx} = \frac{dy/dt}{dx/dt} = -\frac{32t}{50}.
$$

![figure 2.6.2](/calculus/img/keisler/f2.6.2.gif)

**Figure 2.6.2**

### EXAMPLE 7

A particle moves according to the parametric equations

$$
x = t^3 - t,\ \ y = t^2.
$$

Find the slope of its path.

$$
\frac{dx}{dt} = 3t^2 - 1, \ \ \frac{dy}{dt} = 2t,
$$

so

$$
\frac{dy}{dx} = \frac{dy/dt}{dx/dt} = \frac{2t}{3t^2 - 1},\ \ t \ne \pm\sqrt{1 / 3}.
$$

We see from Figure 2.6.3 that the path of this particle is not the graph of a function, and in fact contains a loop and crosses the point \\((0,1)\\) twice, at \\(t = -1\\) and \\(t = 1\\). The path is vertical at the points \\(t = \pm\sqrt{1 / 3}\\), where there is no slope. At the point \\((0,1)\\), the two slopes of the path are \\(dy/dx = -1\\) when \\(t = -1\\), and \\(dy/dx = 1\\) when \\(t = 1\\).

![figure 2.6.3](/calculus/img/keisler/f2.6.3.gif)

**Figure 2.6.3**

### EXAMPLE 8

A particle moving according to the parametric equations

$$
x = \cos t, \ \ y = \sin t
$$

will move counterclockwise around the unit circle at one radian per second beginning at the point \\((1, 0)\\), as shown in Figure 2.6.4. Find the slope of its path at time \\(t\\).

![figure 2.6.4](/calculus/img/keisler/f2.6.4.gif)

**Figure 2.6.4**

$$
\frac{dx}{dt} = -\sin t, \ \ \frac{dy}{dt} = \cos t.
$$

The slope is

$$
\frac{dy}{dx} = \frac{dy/dt}{dx/dt} = -\frac{\cos t}{\sin t}.
$$

In terms of \\(x\\) and \\(y\\) the slope is

$$
\frac{dy}{dx} = -\frac{x}{y}.
$$