+++
date = "2017-11-07T13:06:31+08:00"
+++

# 2.8 Implicit Functions

We now turn to the topic of implicit differentiation. We say that \\(y\\) is an _implicit function_ of \\(x\\) if we are given an equation

$$
\sigma(x, y) = \tau(x, y)
$$

which determines \\(y\\) as a function of \\(x\\). An example is \\(x + xy = 2y\\). Implicit differentiation is a way of finding the derivative of \\(y\\) without actually solving for \\(y\\) as a function of \\(x\\). Assume that \\(dy/dx\\) exists. The method has two steps:

_Step 1_

Differentiate both sides of the equation \\(\sigma(x, y) = \tau(x, y)\\) to get a new equation

**(1)**

$$
\frac{d(\sigma(x, y))}{dx} = \frac{d(\tau(x, y))}{dx}.
$$

The Chain Rule is often used in this step.

_Step 2_

Solve the new Equation 1 for \\(dy/dx\\). The answer will usually involve both \\(x\\) and \\(y\\).

In each of the examples below, we assume that \\(dy/dx\\) exists and use implicit differentiation to find the value of \\(dy/dx\\).

### EXAMPLE 1

Given the equation \\(x + xy = 2y\\), find \\(dy/dx\\).

_Step 1_

$$
\frac{d(x + xy)}{dx} = \frac{d(2y)}{dx}.
$$

We find each side by the Sum and Product Rules,

$$
\frac{d(x + xy)}{dx} = \frac{dx + d(xy)}{dx}
$$

$$
= \frac{dx + x\ dy + y\ dx}{dx} = 1 + x\frac{dy}{dx} + y.
$$

$$
\frac{d(2y)}{dx} = 2\frac{dy}{dx}.
$$

Thus our new equation is

$$
1 + x\frac{dy}{dx} + y = 2\frac{dy}{dx}.
$$

_Step2_

Solve for \\(dy/dx\\).

$$
2\frac{dy}{dx} - x\frac{dy}{dx} = 1 + y.
$$

$$
\frac{dy}{dx} = \frac{1 + y}{2 - x}.
$$

We can check our answer by solving the original equation for \\(y\\) and using ordinary differentiation:

$$
x + xy = 2y.
$$

$$
2y - xy = x.
$$

$$
y = \frac{x}{2 - x}.
$$

By the Quotient Rule,

$$
\frac{dy}{dx} = \frac{(2 - x) \cdot 1 - x(-1)}{(2 - x)^2} = \frac{2}{(2 - x)^2}.
$$

A third way to find \\(dy/dx\\) is to solve the original equation for \\(x\\), find \\(dx/dy\\), and then use the Inverse Function Rule.

$$
x + xy = 2y.
$$

$$
x = \frac{2y}{1 + y}.
$$

$$
\frac{dx}{dy} = \frac{(1 + y) \cdot 2 - 2y \cdot 1}{(1 + y)^2} = \frac{2}{(1 + y)^2}.
$$

$$
\frac{dy}{dx} = \frac{1}{2}(1 + y)^2.
$$

To see that our three answers

$$
\frac{dy}{dx} = \frac{1 + y}{2 - x},
$$

$$
\frac{dy}{dx} = \frac{2}{(2 - x)^2},
$$

$$
\frac{dy}{dx} = \frac{1}{2}(1 + y)^2
$$

are all the same we substitute \\(\frac{x}{2 - x}\\) for \\(y\\):

$$
\frac{dy}{dx} = \frac{1 + y}{2 - x} = \frac{1 + \frac{x}{2 - x}}{2 - x} = \frac{2}{(2 - x)^2}.
$$

$$
\frac{dy}{dx} = \frac{1}{2}(1 + y)^2
$$

$$
= \frac{1}{2}\Bigl(1 + \frac{x}{2 - x}\Bigr)^2 = \frac{2}{(2 - x)^2}.
$$

In Example 1, we found \\(dy/dx\\) by three different methods.

(a) Implicit differentiation. We get \\(dy/dx\\) in terms of both \\(x\\) and \\(y\\).

(b) Solve for \\(y\\) as a function of \\(x\\) and differentiate directly. This gives \\(dy/dx\\) in terms of \\(x\\) only.

\(c) Solve for \\(x\\) as a function of \\(y\\), find \\(dx/dy\\) directly, and use the Inverse Function Rule. This method gives \\(dy/dx\\) in terms of \\(y\\) only.

### EXAMPLE 2

Given \\(y + \sqrt{y} = x^2\\), find \\(dy/dx\\).

$$
\frac{d(y + \sqrt{y})}{dx} = \frac{d(x^2)}{dx}.
$$

$$
\frac{dy}{dx} + \frac{1}{2}y^{-1 / 2}\frac{dy}{dx} = 2x.
$$

$$
\frac{dy}{dx} = \frac{2x}{1 + \frac{1}{2}y^{-1 / 2}}.
$$

This answer can be used to find the slope at any point on the curve, For example, at the point \\((\sqrt{2}, 1)\\) the slope is

$$
\frac{2\sqrt{2}}{1 + \frac{1}{2} \cdot 1^{-1 / 2}} = \frac{2\sqrt{2}}{3 / 2} = \frac{4\sqrt{2}}{3}
$$

while at the point \\((-\sqrt{2}, 1)\\) the slope is

$$
\frac{2(-\sqrt{2})}{1 + \frac{1}{2} \cdot 1^{-1 / 2}} = \frac{-4\sqrt{2}}{3}.
$$

To get \\(dy/dx\\) in terms of \\(x\\), we solve the original equation for \\(y\\) using the quadratic formula:

$$
y + \sqrt{y} - x^2 = 0,
$$

$$
\sqrt{y} = \frac{-1 \pm \sqrt{1 + 4x^2}}{2}.
$$

Since \\(\sqrt{y} \ge 0\\), only one solution may occur,

$$
\sqrt{y} = \frac{-1 + \sqrt{1 + 4x^2}}{2}.
$$

Then

$$
y = \Bigl(\frac{-1 + \sqrt{1 + 4x^2}}{2}\Bigr)^2
$$

The graph of this function is shown in Figure 2.8.1. By substitution we get

$$
\frac{dy}{dx} = \frac{2x}{1 + \frac{1}{2}y^{-1 / 2}}
$$

$$
= \frac{2x}{1 + (-1 + \sqrt{1 + 4x^2})^{-1}}.
$$

![figure 2.8.1](/calculus/img/keisler/f2.8.1.gif)

**Figure 2.8.1**

Often one side of an implicit function equation is constant and has derivative zero.

### EXAMPLE 3

Given \\(x^2 - 2y^2 = 4\\), \\(y \le 0\\), find \\(dy/dx\\).

$$
\frac{d(x^2 - 2y^2)}{dx} = \frac{d(4)}{dx}.
$$

$$
\frac{d(x^2 - 2y^2)}{dx} = 2x - 4y\frac{dy}{dx}.
$$

$$
\frac{d(4)}{dx} = 0.
$$

$$
2x - 4y\frac{dy}{dx} = 0.
$$

$$
\frac{dy}{dx} = \frac{-2x}{-4y} = \frac{x}{2y}.
$$

Solving the original equation for \\(y\\), we get

$$
-2y^2 = 4 - x^2, \ \ y \le 0;
$$

$$
y^2 = \frac{x^2 - 4}{2}, \ \ y \le 0;
$$

$$
y = -\sqrt{\frac{x^2 - 4}{2}}.
$$

Thus \\(dy/dx\\) in terms of \\(x\\) is

$$
\frac{dy}{dx} = \frac{x}{2y}
$$

$$
= \frac{x}{-2\sqrt{\frac{x^2 - 4}{2}}} = - \frac{x}{\sqrt{2(x^2 - 4)}}.
$$

The graph of this function is shown in Figure 2.8.2.

![figure 2.8.2](/calculus/img/keisler/f2.8.2.gif)

**Figure 2.8.2**

Implicit differentiation can even be applied to an equation that does not by itself determine \\(y\\) as a function \\(x\\). Sometimes extra inequalities must be assumed in order to make \\(y\\) a function of \\(x\\).

### EXAMPLE 4

Given

**(2)**

$$
x^2 + y^2 = 1,
$$

find \\(dy/dx\\). This equation does not determine \\(y\\) as a function of \\(x\\); its graph is the unit circle. Nevertheless we differentiate both sides with respect to \\(x\\) and solve for \\(dy/dx\\).

$$
2x + 2y\frac{dy}{dx} = 0, \ \ \frac{dy}{dx} = -\frac{x}{y}.
$$

We can conclude that for any system of formulas S which contains the Equation 2 and also determines \\(y\\) as a function of \\(x\\), it is true that

**(3)**

$$
\frac{dy}{dx} = -\frac{x}{y}.
$$

We can use Equation 3 to find the slope of the line tangent to the unit circle at any point on the circle. The following examples are illustrated in Figure 2.8.3.

![figure 2.8.3](/calculus/img/keisler/f2.8.3.gif)

**Figure 2.8.3**

$$
\frac{dy}{dx} = 0 \ at \ (0, -1),
$$

$$
\frac{dy}{dx} = -\frac{1}{\sqrt{3}} \ at \ (\frac{1}{2}, \frac{\sqrt{3}}{2}),
$$

$$
\frac{dy}{dx} = \sqrt{8} \ at \ (\frac{\sqrt{8}}{3}, -\frac{1}{3}),
$$

$$
\frac{dy}{dx}\ {is\ undefined\ at}\ (-1, 0).
$$

The system of formulas

$$
x^2 + y^2 = 1,\ \ y \ge 0
$$

gives us

$$
y = \sqrt{1 - x^2}, \ \ \frac{dy}{dx} = -\frac{x}{y} = -\frac{x}{\sqrt{1 - x^2}}.
$$

On the other hand the system

$$
x^2 + y^2 = 1,\ \ y \le 0
$$

gives us

$$
y = -\sqrt{1 - x^2}, \ \ \frac{dy}{dx} = -\frac{x}{y} = \frac{x}{\sqrt{1 - x^2}}.
$$

### EXAMPLE 5

Find the slope of the line tangent to the curve

**(4)**

$$
x^5y^3 + xy^6 = y + 1
$$

at the points \\((1,1)\\), \\((1, -1)\\), and \\((0, -1)\\).

The three points are all on the curve, and the first two points have the same \\(x\\) coordinate, so Equation 4 does not by itself determine \\(y\\) as a function of \\(x\\).

We differentiate with respect to \\(x\\),

$$
\frac{d(x^5y^3 + xy^6)}{dx} = \frac{d(y + 1)}{dx}.
$$

$$
5x^4y^3 + x^5 \cdot 3y^2\frac{dy}{dx} + y^6 + 6xy^5\frac{dy}{dx} = \frac{dy}{dx},
$$

and then solve for \\(dy/dx\\),

$$
5x^4y^3 + y^6 + (3x^5y^2 + 6xy^5 - 1)\frac{dy}{dx} = 0,
$$

**(5)**

$$
\frac{dy}{dx} = -\frac{5x^4y^3 +y^6}{3x^5y^2 + 6xy^5 - 1}.
$$

Substituting,

$$
\frac{dy}{dx} = -\frac{6}{8} \ at \ (1, 1).
$$

$$
\frac{dy}{dx} = -1 \ at \ (1, -1).
$$

$$
\frac{dy}{dx} = +1 \ at \ (0, -1).
$$

Equation 5 for \\(dy/dx\\) is true of any system \\(S\\) of formulas which contains Equation 4 and determines \\(y\\) as a function of \\(x\\).

Here is what generally happens in the method of implicit differentiation. Given an equation

**(6)**

$$
\tau(x,y) = \sigma(x,y)
$$

between two terms which may involve the variables \\(x\\) and \\(y\\), we differentiate both sides of the equation and obtain

**(7)**

$$
\frac{d(\tau(x,y))}{dx} = \frac{d(\sigma(x,y))}{dx}.
$$

We then solve Equation 7 to get \\(dy/dx\\) equal to a term which typically involves both \\(x\\) and \\(y\\). We can conclude that for any system of formulas which contains Equation 6 and determines \\(y\\) as a function of \\(x\\). Equation 7 is true. Also, Equation 7 can be used to find the slope of the tangent line at any point on the curve \\(\tau(x, y) = \sigma(x, y)\\).
