+++
date = "2017-10-28T13:12:00+08:00"
categories = ["math", "calculus"]
tags = ["differentiation", "derivative"]
title = "2.3 Derivatives of Rational Functions"
url = "calculus/keisler/02/03/"
+++

A term of the form

$$
a_1x + a_0
$$

where \\(a_1, a_0\\) are real numbers, is called a _linear term_ in \\(x\\); if \\(a_1 \ne 0\\), it is also called _polynomial of degree one_ in \\(x\\). A term of the form

$$
a_2x^2 + a_1x + a_0, a_2 \ne 0
$$

is called a _polynomial of degree two_ in \\(x\\), and, in general, a term of the form

$$
a_nx^n + a\_{n-1} x^{n-1} + \cdots + a_1x + a_0, a_n \ne 0
$$

is called a _polynomial of degree n_ in \\(x\\).

A _rational term_ in \\(x\\) is any term which is built up from the variable \\(x\\) and real numbers using the operations of addition, multiplication, subtraction, and division. For example every polynomial is a rational term and so are the terms

$$
\frac{(3x^2 - 5)(x + 2)^3}{5x - 11}, \frac{(1 + 1/x)^9}{x^3 + 1/(2 - x)}. 
$$

A _linear function_, _polynomial function_, or _rational function_ is a function which is given by a linear term, polynomial, or rational term, respectively. In this section we shall establish a set of rules which enable us to quickly differentiate any rational function. The rules will also be useful later on in differentiating other functions.

**THEOREM 1**

_The derivative of a linear function is equal to the coefficient of \\(x\\). That is,_

$$
\frac{d(bx + c)}{dx} = b, d(bx + c) = b\ dx.
$$

_PROOF_

Let \\(y = bx + c\\), and let \\(\Delta{x} \ne 0\\) be infinitesimal. Then

$$
y + \Delta{y} = b(x + \Delta{x}) + c,
$$

$$
\Delta{y} = (b(x + \Delta{x}) + c) - (bx + c) = b\ \Delta{x},
$$

$$
\frac{\Delta{y}}{\Delta{x}} = \frac{b\ \Delta{x}}{\Delta{x}} = b.
$$

Therefore

$$
\frac{dy}{dx} = st(b) = b.
$$

Multiplying through by \\(dx\\), we obtain at once

$$
dy = b\ dx.
$$

If in Theorem 1 we put \\(b = 1, c = 0\\), we see that the derivative of the identity function \\(f(x) = x\\) is \\(f^\prime(x) = 1
\\); i.e.,

$$
\frac{dx}{dx} = 1,\ dx = dx.
$$

On the other hand, if we put \\(b = 0\\) in Theorem 1 then the term \\(bx + c\\) is just the constant \\(c\\), and we find that the derivative of the constant function \\(f(x) = c\\) is \\(f^\prime(x) = 0\\); i.e.,

$$
\frac{dc}{dx} = 0,\ dc = 0.
$$

**THEOREM 2 (Sum Rule)**

_Suppose \\(u\\) and \\(v\\) depend on the independent variable \\(x\\). Then for any value of \\(x\\) where \\(du/dx\\) and \\(dv/dx\\) exist,_

$$
\frac{d(u + v)}{dx} = \frac{du}{dx} + \frac{dv}{dx},\ d(u + v) = du + dv.
$$

In other words, the derivative of the sum is the sum of the derivatives.

_PROOF_

Let \\(y = u + v\\), and let \\(\Delta{x} \ne 0\\) be infinitesimal. Then

$$
y + \Delta{y} = (u + \Delta{u}) + (v + \Delta{v}),
$$

$$
\Delta{y} = [(u + \Delta{u}) + (v + \Delta{v})] - [u + v] = \Delta{u} + \Delta{v},
$$

$$
\frac{\Delta{y}}{\Delta{x}} = \frac{\Delta{u} + \Delta{v}}{\Delta{x}} = \frac{\Delta{u}}{\Delta{x}} + \frac{\Delta{v}}{\Delta{x}}.
$$

Taking standard parts,

$$
st\Bigl(\frac{\Delta{y}}{\Delta{x}}\Bigr) = st\Bigl(\frac{\Delta{u}}{\Delta{x}} + \frac{\Delta{v}}{\Delta{x}}\Bigr) = st\Bigl(\frac{\Delta{u}}{\Delta{x}}\Bigr) + st\Bigl(\frac{\Delta{v}}{\Delta{x}}\Bigr).
$$

Thus

$$
\frac{dy}{dx} = \frac{du}{dx} + \frac{dv}{dx}.
$$

By using the Sum Rule \\(n - 1\\) times, we see that

$$
\frac{d(u_1 + \cdots + u_n)}{dx} = \frac{du_1}{dx} + \cdots + \frac{du_n}{dx},
$$

or

$$
d(u_1 + \cdots + u_n) = du_1 + \cdots + du_n.
$$

**THEOREM 3 (Constant Rule)**

_Suppose \\(u\\) depends on \\(x\\), and \\(c\\) is a real number. Then for any value of \\(x\\) where \\(du/dx\\) exists,_

$$
\frac{d(cu)}{dx} = c\frac{du}{dx},\ d(cu) = c\ du.
$$

_PROOF_

Let \\(y = cu\\), and let \\(\Delta{x} \ne 0\\) be infinitesimal. Then

$$
y + \Delta{y} = c(u + \Delta{u}),
$$

$$
\Delta{y} = c(u + \Delta{u}) - cu = c\ \Delta{u},
$$

$$
\frac{\Delta{y}}{\Delta{x}} = \frac{c\ \Delta{u}}{\Delta{x}} = c\frac{\Delta{u}}{\Delta{x}}.
$$

Taking standard parts,

$$
st\Bigl(\frac{\Delta{y}}{\Delta{x}}\Bigr) = st\Bigl(c\frac{\Delta{u}}{\Delta{x}}\Bigr) = c\ st\Bigl(\frac{\Delta{u}}{\Delta{x}}\Bigr)
$$

whence

$$
\frac{dy}{dx} = c\ \frac{du}{dx}.
$$

The Constant Rule shows that in computing derivatives, a constant factor may be moved "outside" the derivative. It can only be used when \\(c\\) is a constant. For products of two functions of \\(x\\), we have:

**THEOREM 4 (Product Rule)**

_Suppose \\(u\\) and \\(v\\) depend on \\(x\\). Then for any value of \\(x\\) where \\(du/dx\\) and \\(dv/dx\\) exist,_

$$
\frac{d(uv)}{dx} = u\frac{dv}{dx} + v\frac{du}{dx},
$$

$$
d(uv) = u\ dv + v\ du.
$$

_PROOF_

Let \\(y = uv\\), and let \\(\Delta{x} \ne 0\\) be infinitesimal.

$$
y + \Delta{y} = (u + \Delta{u})(v + \Delta{v}),
$$

$$
\Delta{y} = (u + \Delta{u})(v + \Delta{v}) - uv
$$

$$
= u\ \Delta{v} + v\ \Delta{u} + \Delta{u}\ \Delta{v},
$$

$$
\frac{\Delta{y}}{\Delta{x}} = \frac{u\ \Delta{v} + v\ \Delta{u} + \Delta{u}\ \Delta{v}}{\Delta{x}}
$$

$$
= u\frac{\Delta{v}}{\Delta{x}} + v\frac{\Delta{u}}{\Delta{x}} + \Delta{u}\frac{\Delta{v}}{\Delta{x}}.
$$

\\(\Delta{u}\\) is infinitesimal by the Increment Theorem, whence

$$
st\Bigl(\frac{\Delta{y}}{\Delta{x}}\Bigr) = st\Bigl(u\frac{\Delta{v}}{\Delta{x}} + v\frac{\Delta{u}}{\Delta{x}} + \Delta{u}\frac{\Delta{v}}{\Delta{x}}\Bigr)
$$

$$
= u \cdot st\Bigl(\frac{\Delta{v}}{\Delta{x}}\Bigr) + v \cdot st\Bigl(\frac{\Delta{u}}{\Delta{x}}\Bigr) + 0 \cdot st\Bigl(\frac{\Delta{v}}{\Delta{x}}\Bigr)
$$

So

$$
\frac{dy}{dx} = u\frac{dv}{dx} + v\frac{du}{dx}.
$$

The Constant Rule is really the special case of the Product Rule where \\(v\\) is a constant function of \\(x, v = c\\). To check this we let \\(v\\) be the constant \\(c\\) and see what the Product Rule gives us:

$$
\frac{d(u \cdot c)}{dx} = u\frac{dc}{dx} + c\frac{du}{dx}
$$

$$
= u \cdot 0 + c\frac{du}{dx} = c\frac{du}{dx}.
$$

This is the Constant Rule.

The Product Rule can also be used to find the derivative of a power of \\(u\\).

**THEOREM 5 (Power Rule)**

_Let \\(u\\) depend on \\(x\\) and let \\(n\\) be a positive integer. For any value of \\(x\\) where \\(du/dx\\) exists,_

$$
\frac{d(u^n)}{dx} = nu^{n-1}\frac{du}{dx}, d(u^n) = nu^{n-1}\ du.
$$

_PROOF_

To see what is going on we first prove the Power Rule for \\(n = 1, 2, 3, 4\\).

\\(n = 1\\): We have \\(u^n = u\\) and \\(u^0 = 1\\), whence

$$
\frac{d(u^n)}{dx} = \frac{du}{dx} = 1 \cdot u^0 \cdot \frac{du}{dx}.
$$

\\(n = 2\\): We use the Product Rule,

$$
\frac{d(u^2)}{dx} = \frac{d(u \cdot u)}{dx} = u\frac{du}{dx} + u\frac{du}{dx} = 2 \cdot u^1 \cdot \frac{du}{dx}.
$$

\\(n = 3\\): We write \\(u^3 = u \cdot u^2\\), use the Product Rule again, and then use the result for \\(n = 2\\).

$$
\frac{d(u^3)}{dx} = \frac{d(u \cdot u^2)}{dx} = u\frac{d(u^2)}{dx} + u^2\frac{du}{dx}
$$

$$
= u \cdot 2u \frac{du}{dx} + u^2 \frac{du}{dx} = 3u^2 \frac{du}{dx}.
$$

\\(n = 4\\): Using the Product Rule and then the result for \\(n = 3\\),

$$
\frac{d(u^4)}{dx} = \frac{d(u \cdot u^3)}{dx} = u\frac{d(u^3)}{dx} + u^3\frac{du}{dx}
$$

$$
= u \cdot 3u^2 \frac{du}{dx} + u^3 \frac{du}{dx} = 4u^3 \frac{du}{dx}.
$$

We can continue this process indefinitely and prove the theorem for every positive integer \\(n\\). To see this, assume that we have proved the theorem for \\(m\\). That is, assume that

**(1)**

$$
\frac{d(u^m)}{dx} = mu^{m-1}\frac{du}{dx}.
$$

We then show that it is also true for \\(m + 1\\). Using the Product Rule and the Equation 1,

$$
\frac{d(u^{m+1})}{dx} = \frac{d(u \cdot u^m)}{dx} = u\frac{d(u^m)}{dx} + u^m\frac{du}{dx}
$$

$$
= u \cdot mu^{m-1} \frac{du}{dx} + u^m \frac{du}{dx} = (m+1)u^m\frac{du}{dx}.
$$

Thus

$$
\frac{d(u^{m+1})}{dx} = (m+1)u^m\frac{du}{dx}.
$$

This shows that the theorem holds for \\(m + 1\\).

We have shown the theorem is true for \\(1, 2, 3, 4\\). Set \\(m = 4\\); then the theorem holds for \\(m + 1 = 5\\). Set \\(m = 5\\); then it holds for \\(m + 1 = 6\\). And so on. Hence the theorem is true for all positive integers \\(n\\).

In the proof of the Power Rule, we used the following principle:

**PRINCIPLE OF INDUCTION**

_Suppose a statement \\(P(n)\\) about an arbitrary integer \\(n\\) is true when \\(n = 1\\). Suppose further that for any positive integer \\(m\\) such that \\(P(m)\\) is true, \\(P(m + 1)\\) is also true. Then the statement \\(P(n)\\) is true of every positive integer \\(n\\)._

In the previous proof, \\(P(n)\\) was the Power Rule,

$$
\frac{d(u^n)}{dx} = nu^{n-1}\frac{du}{dx}.
$$

The Principle of Induction can be made plausible in the following way. Let a positive integer \\(n\\) be given. Set \\(m = 1\\); since \\(P(1)\\) is true, \\(P(2)\\) is true. Now set \\(m = 2\\); since \\(P(2)\\) is true, \\(P(3)\\) is true. We continue reasoning in this way for \\(n\\) steps and conclude that \\(P(n)\\) is true.

The Power Rule also holds for \\(n = 0\\) because when \\(u \ne 0, u^0 = 1\\) and \\(d1/dx = 0\\).

Using the Sum, Constant, and Power rules, we can compute the derivative of a polynomial function very easily. We have

$$
\frac{d(x^n)}{dx} = nx^{n-1},
$$

$$
\frac{d(cx^n)}{dx} = cnx^{n-1},
$$

and thus

$$
\frac{d(a_nx^n + a\_{n-1}x^{n-1} + \cdots + a_1x + a_0)}{dx}
$$

$$
= a_n \cdot nx^{n-1} + a\_{n-1}(n-1)x^{n-2} + \cdots + a_1.
$$

**EXAMPLE 1**

$$
\frac{d(-3x^5)}{dx} = -3 \cdot 5x^4 = -15x^4.
$$

**EXAMPLE 2**

$$
\frac{d(6x^4 - 2x^3 + x - 1)}{dx} = 24x^3 - 6x^2 + 1.
$$

Two useful facts can be stated as corollaries.

**COROLLARY 1**

_The derivative of a polynomial of degree \\(n > 0\\) is a polynomial of degree \\(n - 1\\). (A nonzero constant is counted as a polynomial of degree zero.)_

**COROLLARY 2**

_If \\(u\\) depends on \\(x\\), then_

$$
\frac{d(u + c)}{dx} = \frac{du}{dx}
$$

_whenever \\(du/dx\\) exists. That is, adding a constant to a function does not change its derivative._

In Figure 2.3.1 we see that the effect of adding a constant is to move the curve up or down the y-axis without changing the slope.

![figure 2.3.1](/img/calculus/keisler/f2.3.1.gif)

**Figure 2.3.1**

For the last two rules in this section we need the formula for the derivative of \\(1/v\\).

**LEMMA**

_Suppose \\(v\\) depends on \\(x\\). Then for any value of \\(x\\) where \\(v \ne 0\\) and \\(dv/dx\\) exists,_

$$
\frac{d(1/v)}{dx} = -\frac{1}{v^2}\frac{dv}{dx},\ d\Bigl(\frac{1}{v}\Bigr) = -\frac{1}{v^2}dv.
$$